agda/STLC/Test.agda
@@ -1,0 +1,65 @@
+module STLC.Test where
+
+open import STLC.Prelude
+
+data Type : Set where
+  Int : Type
+  Top : Type
+  _⇒_ : Type → Type → Type
+  _&_ : Type → Type → Type
+
+-- a isomorphic relation between types --
+
+data _⇠_⇢_ : Type → Type → Type → Set where
+
+  sp-and : ∀ {A B}
+    → A ⇠ (A & B) ⇢ B
+
+  sp-arr : ∀ {A B B₁ B₂}
+    → B₁ ⇠ B ⇢ B₂
+    → (A ⇒ B₁) ⇠ (A ⇒ B) ⇢ (A ⇒ B₂)
+
+data _≲_ : Type → Type → Set where
+
+  ≲-refl : ∀ {A}
+    → A ≲ A
+
+  ≲-and : ∀ {A₁ A₂ B B₁ B₂}
+    → B₁ ⇠ B ⇢ B₂
+    → A₁ ≲ B₁
+    → A₂ ≲ B₂
+    → (A₁ & A₂) ≲ B
+
+size : Type → ℕ
+size Int = 1
+size Top = 1
+size (A ⇒ B) = 1 + size A + size B
+size (A & B) = 1 + size A + size B
+
+size>0 : ∀ A
+  → size A > 0
+size>0 Int = s≤s z≤n
+size>0 Top = s≤s z≤n
+size>0 (A ⇒ A₁) = s≤s z≤n
+size>0 (A & A₁) = s≤s z≤n
+
+≲-trans-k : ∀ {A B C k}
+  → size B < k
+  → A ≲ B
+  → B ≲ C
+  → A ≲ C
+≲-trans-k {B = Int} {k = suc k} (s≤s sz) ≲-refl BC = BC
+≲-trans-k {B = Top} {k = suc k} sz ≲-refl BC = BC
+≲-trans-k {B = B₁ ⇒ B₂} {k = suc k} (s≤s sz) AB ≲-refl = AB
+≲-trans-k {B = B₁ & B₂} {k = suc k} (s≤s sz) AB ≲-refl = AB
+≲-trans-k {B = B₁ & B₂} {k = suc k} (s≤s sz) ≲-refl (≲-and x BC BC₁) = ≲-and x BC BC₁
+≲-trans-k {B = B₁ & B₂} {k = suc k} (s≤s sz) (≲-and sp-and AB AB₁) (≲-and x BC BC₁) =
+  ≲-and x
+    (≲-trans-k {k = k} (<-trans (m<m+n (size B₁) (size>0 B₂)) sz) AB BC)
+    (≲-trans-k {k = k} (<-trans (m<n+m (size B₂) (size>0 B₁)) sz) AB₁ BC₁)
+
+≲-trans : ∀ {A B C}
+  → A ≲ B
+  → B ≲ C
+  → A ≲ C
+≲-trans {B = B} = ≲-trans-k (n<1+n (size B))
